@prefix bmo: <https://bbp.epfl.ch/ontologies/core/bmo/> .
@prefix efe: <https://bbp.epfl.ch/ontologies/core/efeatures/> .
@prefix nsg: <https://neuroshapes.org/> .
@prefix owl: <http://www.w3.org/2002/07/owl#> .
@prefix rdfs: <http://www.w3.org/2000/01/rdf-schema#> .
@prefix skos: <http://www.w3.org/2004/02/skos/core#> .
@prefix xsd: <http://www.w3.org/2001/XMLSchema#> .

skos:altLabel a owl:AnnotationProperty .

skos:definition a owl:AnnotationProperty .

bmo:Other a owl:Class ;
    rdfs:label "Other"@en ;
    rdfs:subClassOf bmo:NeuronElectrophysiologicalFeature,
        efe:NeuroElectroNeuronElectrophysiologicalFeature ;
    skos:altLabel "Other"@en ;
    skos:definition "A catch-all property to reflect any properties which are not already explicitly defined"@en ;
    nsg:units "Unitless" .

<https://bbp.epfl.ch/ontologies/core/efeatures> a owl:Ontology ;
    rdfs:label "Electrophysiological Features Ontology"@en ;
    owl:versionInfo "R249"^^xsd:string .

efe:ADPAmplitude a owl:Class ;
    rdfs:label "ADP Amplitude"@en ;
    rdfs:subClassOf bmo:NeuronElectrophysiologicalFeature,
        efe:NeuroElectroNeuronElectrophysiologicalFeature ;
    skos:definition "Amplitude from first AP onset to maximum voltage, typically more depolarized than the resting membrane potential"@en ;
    nsg:units "mV" .

efe:ADPDuration a owl:Class ;
    rdfs:label "ADP Duration"@en ;
    rdfs:subClassOf bmo:NeuronElectrophysiologicalFeature,
        efe:NeuroElectroNeuronElectrophysiologicalFeature ;
    skos:definition "Duration from first AP onset to maximum ADP"@en ;
    nsg:units "ms" .

efe:AHPAmplitude a owl:Class ;
    rdfs:label "AHP Amplitude"@en ;
    rdfs:subClassOf bmo:NeuronElectrophysiologicalFeature,
        efe:NeuroElectroNeuronElectrophysiologicalFeature ;
    skos:definition "Calculated as the voltage difference between AP threshold and AP trough. Commonly defined using first AP in train at rheobase current."@en ;
    nsg:units "mV" .

efe:AHPAmplitudeFromResting a owl:Class ;
    rdfs:label "AHP Amplitude From Resting"@en ;
    rdfs:subClassOf bmo:NeuronElectrophysiologicalFeature,
        efe:NeuroElectroNeuronElectrophysiologicalFeature ;
    skos:definition "Calculated as the voltage difference between resting or baseline voltages and AP trough. Commonly defined using first AP in train at rheobase current."@en ;
    nsg:units "mV" .

efe:AHPDepth a owl:Class ;
    rdfs:label "AHP Depth"@en ;
    rdfs:subClassOf bmo:NeuronElectrophysiologicalFeature ;
    skos:definition "Relative voltage values at the first after-hyperpolarization."^^xsd:string ;
    efe:efel_id "AHP_depth"^^xsd:string ;
    efe:efel_namespace "LibV1"^^xsd:string ;
    nsg:units "mV"^^xsd:string .

efe:AHPDepthAbs a owl:Class ;
    rdfs:label "AHP Depth Abs"@en ;
    rdfs:subClassOf bmo:NeuronElectrophysiologicalFeature ;
    skos:definition "Absolute voltage values at the first after-hyperpolarization."^^xsd:string ;
    efe:efel_id "AHP_depth_abs"^^xsd:string ;
    efe:efel_namespace "LibV1"^^xsd:string ;
    nsg:units "mV"^^xsd:string .

efe:AHPDepthAbsSlow a owl:Class ;
    rdfs:label "AHP Depth Abs Slow"@en ;
    rdfs:subClassOf bmo:NeuronElectrophysiologicalFeature ;
    skos:definition "Absolute voltage values at the first after-hyperpolarization starting a given number of ms (default: 5) after the peak."^^xsd:string ;
    efe:efel_id "AHP_depth_abs_slow"^^xsd:string ;
    efe:efel_namespace "LibV1"^^xsd:string ;
    nsg:units "mV"^^xsd:string .

efe:AHPDuration a owl:Class ;
    rdfs:label "AHP Duration"@en ;
    rdfs:subClassOf bmo:NeuronElectrophysiologicalFeature,
        efe:NeuroElectroNeuronElectrophysiologicalFeature ;
    skos:definition "Duration of AP after-hyperpolarization, not explicitly referred to by author as either fast or slow"@en ;
    nsg:units "ms" .

efe:AHPSlowTime a owl:Class ;
    rdfs:label "AHP Slow Time"@en ;
    rdfs:subClassOf bmo:NeuronElectrophysiologicalFeature ;
    skos:definition "Time difference between slow AHP (see AHP Depth Abs Slow) and peak, divided by interspike interval."^^xsd:string ;
    efe:efel_id "AHP_slow_time"^^xsd:string ;
    efe:efel_namespace "LibV1"^^xsd:string ;
    nsg:units "ms"^^xsd:string .

efe:AHPTimeFromPeak a owl:Class ;
    rdfs:label "AHP Time From Peak"@en ;
    rdfs:subClassOf bmo:NeuronElectrophysiologicalFeature ;
    skos:definition "Time between AP peaks and first AHP depths"^^xsd:string ;
    efe:efel_id "AHP_time_from_peak"^^xsd:string ;
    efe:efel_namespace "LibV5"^^xsd:string ;
    nsg:units "mV"^^xsd:string .

efe:AHPVoltage a owl:Class ;
    rdfs:label "AHP Voltage"@en ;
    rdfs:subClassOf bmo:NeuronElectrophysiologicalFeature,
        efe:NeuroElectroNeuronElectrophysiologicalFeature ;
    skos:definition "Calculated as minimum voltage value during an AHP. Commonly defined using first AP in train at rheobase current."@en ;
    nsg:units "mV" .

efe:AP1Width a owl:Class ;
    rdfs:label "AP1 Width"@en ;
    rdfs:subClassOf bmo:NeuronElectrophysiologicalFeature ;
    skos:definition "Width of the first spike at threshold"^^xsd:string ;
    efe:efel_id "AP1_width"^^xsd:string ;
    efe:efel_namespace "LibV5"^^xsd:string ;
    nsg:units "ms"^^xsd:string .

efe:AP2Width a owl:Class ;
    rdfs:label "AP2 Width"@en ;
    rdfs:subClassOf bmo:NeuronElectrophysiologicalFeature ;
    skos:definition "Width of the second spike at threshold"^^xsd:string ;
    efe:efel_id "AP2_width"^^xsd:string ;
    efe:efel_namespace "LibV5"^^xsd:string ;
    nsg:units "ms"^^xsd:string .

efe:APAmplitude a owl:Class ;
    rdfs:label "AP Amplitude"@en ;
    rdfs:subClassOf bmo:NeuronElectrophysiologicalFeature ;
    skos:definition "The relative height of the action potential from spike onset."^^xsd:string ;
    efe:efel_id "AP_Amplitude"^^xsd:string ;
    efe:efel_namespace "LibV1"^^xsd:string ;
    nsg:units "mV"^^xsd:string .

efe:APDurationHalfWidth a owl:Class ;
    rdfs:label "AP Duration Half Width"@en ;
    rdfs:subClassOf bmo:NeuronElectrophysiologicalFeature ;
    skos:definition "Width of spike at half spike amplitude."^^xsd:string ;
    efe:efel_id "AP_duration_half_width"^^xsd:string ;
    efe:efel_namespace "LibV2"^^xsd:string ;
    nsg:units "ms"^^xsd:string .

efe:APRiseTime a owl:Class ;
    rdfs:label "AP Rise Time"@en ;
    rdfs:subClassOf bmo:NeuronElectrophysiologicalFeature ;
    skos:definition "Time between the AP threshold and the peak, given a window (default: from 0% to 100% of the AP amplitude)"^^xsd:string ;
    efe:efel_id "AP_rise_time"^^xsd:string ;
    efe:efel_namespace "LibV2"^^xsd:string ;
    nsg:units "ms"^^xsd:string .

efe:AccessResistance a owl:Class ;
    rdfs:label "Access Resistance"@en ;
    rdfs:subClassOf bmo:NeuronElectrophysiologicalFeature,
        efe:NeuroElectroNeuronElectrophysiologicalFeature ;
    skos:definition "Sum of the electrode resistance and the resistance at the electrode-cell junction"@en ;
    nsg:units "M\\ohm" .

efe:AdaptationPercent1 a owl:Class ;
    rdfs:label "Adaptation Percent1"@en ;
    rdfs:subClassOf bmo:NeuronElectrophysiologicalFeature,
        efe:NeuroElectroNeuronElectrophysiologicalFeature ;
    skos:altLabel "adaptation percent (first/last ISI)"@en ;
    skos:definition "Percentage of durations between early and late AP inter-spike intervals in an AP train"@en ;
    nsg:units "Unitless" .

efe:AdaptationPercent2 a owl:Class ;
    rdfs:label "Adaptation Percent2"@en ;
    rdfs:subClassOf bmo:NeuronElectrophysiologicalFeature,
        efe:NeuroElectroNeuronElectrophysiologicalFeature ;
    skos:altLabel "adaptation percent (last/first ISI)"@en ;
    skos:definition "Percentage of durations between late and early AP inter-spike intervals in an AP train"@en ;
    nsg:units "Unitless" .

efe:AdaptationPercent3 a owl:Class ;
    rdfs:label "Adaptation Percent3"@en ;
    rdfs:subClassOf bmo:NeuronElectrophysiologicalFeature,
        efe:NeuroElectroNeuronElectrophysiologicalFeature ;
    skos:altLabel "adaptation percent (1 - first/last ISI)"@en ;
    skos:definition "1 minus ratio of durations between early and late AP inter-spike intervals in an AP train, normalized to a percent"@en ;
    nsg:units "Unitless" .

efe:AdaptationRatio a owl:Class ;
    rdfs:label "Adaptation Ratio"@en ;
    rdfs:subClassOf bmo:NeuronElectrophysiologicalFeature,
        efe:NeuroElectroNeuronElectrophysiologicalFeature ;
    skos:definition "Ratio of durations between early and late AP inter-spike intervals in an AP train"@en ;
    nsg:units "Unitless" .

efe:AdaptationRatio1 a owl:Class ;
    rdfs:label "Adaptation Ratio1"@en ;
    rdfs:subClassOf bmo:NeuronElectrophysiologicalFeature,
        efe:NeuroElectroNeuronElectrophysiologicalFeature ;
    skos:altLabel "adaptation ratio (last/first ISI)"@en ;
    skos:definition "Ratio of durations between late and early AP inter-spike intervals in an AP train"@en ;
    nsg:units "Unitless" .

efe:AdaptationRatio2 a owl:Class ;
    rdfs:label "Adaptation Ratio2"@en ;
    rdfs:subClassOf bmo:NeuronElectrophysiologicalFeature,
        efe:NeuroElectroNeuronElectrophysiologicalFeature ;
    skos:altLabel "adaptation ratio (1 - first/last ISI)"@en ;
    skos:definition "1 minus ratio of durations between early and late AP inter-spike intervals in an AP train"@en ;
    nsg:units "Unitless" .

efe:AdaptationRatio3 a owl:Class ;
    rdfs:label "Adaptation Ratio3"@en ;
    rdfs:subClassOf bmo:NeuronElectrophysiologicalFeature,
        efe:NeuroElectroNeuronElectrophysiologicalFeature ;
    skos:altLabel "adaptation ratio (other)"@en ;
    skos:definition "Adaptation ratio, percent, index but not otherwise characterizable to an existing sub-definition"@en ;
    nsg:units "Unitless" .

efe:BurstNumber a owl:Class ;
    rdfs:label "Burst Number"@en ;
    rdfs:subClassOf bmo:NeuronElectrophysiologicalFeature ;
    skos:definition "The number of bursts."^^xsd:string ;
    efe:efel_id "burst_number"^^xsd:string ;
    efe:efel_namespace "LibV1"^^xsd:string ;
    nsg:units "dimensionless"^^xsd:string .

efe:CellCapacitance a owl:Class ;
    rdfs:label "Cell Capacitance"@en ;
    rdfs:subClassOf bmo:NeuronElectrophysiologicalFeature,
        efe:NeuroElectroNeuronElectrophysiologicalFeature ;
    skos:definition "Neuron capacitance, typically measured by dividing membrane time constant by membrane resistance"@en ;
    nsg:units "pF" .

efe:CellDiameter a owl:Class ;
    rdfs:label "Cell Diameter"@en ;
    rdfs:subClassOf bmo:NeuronElectrophysiologicalFeature,
        efe:NeuroElectroNeuronElectrophysiologicalFeature ;
    skos:definition "Diameter of the cell soma"@en ;
    nsg:units "um" .

efe:CellSurfaceArea a owl:Class ;
    rdfs:label "Cell Surface Area"@en ;
    rdfs:subClassOf bmo:NeuronElectrophysiologicalFeature,
        efe:NeuroElectroNeuronElectrophysiologicalFeature ;
    skos:definition "Cross-sectional area of the cell"@en ;
    nsg:units "m" .

efe:CheckAISInitiation a owl:Class ;
    rdfs:label "Check AIS Initiation"@en ;
    rdfs:subClassOf bmo:NeuronElectrophysiologicalFeature ;
    skos:definition "Check initiation of AP in AIS"^^xsd:string ;
    efe:efel_id "check_AISInitiation"^^xsd:string ;
    efe:efel_namespace "LibV5"^^xsd:string ;
    nsg:units "ms"^^xsd:string .

efe:DecayTimeConstantAfterStim a owl:Class ;
    rdfs:label "Decay Time Constant After Stim"@en ;
    rdfs:subClassOf bmo:NeuronElectrophysiologicalFeature ;
    skos:definition "The decay time constant of the voltage right after the stimulus"^^xsd:string ;
    efe:efel_id "decay_time_constant_after_stim"^^xsd:string ;
    efe:efel_namespace "LibV5"^^xsd:string ;
    nsg:units "ms"^^xsd:string .

efe:FISlope a owl:Class ;
    rdfs:label "FI Slope"@en ;
    rdfs:subClassOf bmo:NeuronElectrophysiologicalFeature,
        efe:NeuroElectroNeuronElectrophysiologicalFeature ;
    skos:definition "Slope of the frequency-current relationship"@en ;
    nsg:units "Hz/nA" .

efe:FastAHPAmplitude a owl:Class ;
    rdfs:label "Fast AHP Amplitude"@en ;
    rdfs:subClassOf bmo:NeuronElectrophysiologicalFeature,
        efe:NeuroElectroNeuronElectrophysiologicalFeature ;
    skos:definition "Calculated as the difference between AP threshold and AP trough, explictly refered to by author as fast."@en ;
    nsg:units "mV" .

efe:FastAHPAmplitudeFromResting a owl:Class ;
    rdfs:label "Fast AHP Amplitude From Resting"@en ;
    rdfs:subClassOf bmo:NeuronElectrophysiologicalFeature,
        efe:NeuroElectroNeuronElectrophysiologicalFeature ;
    skos:definition "Calculated as the difference between resting or baseline voltages and AP trough, explictly refered to by author as fast."@en ;
    nsg:units "mV" .

efe:FastAHPDuration a owl:Class ;
    rdfs:label "Fast AHP Duration"@en ;
    rdfs:subClassOf bmo:NeuronElectrophysiologicalFeature,
        efe:NeuroElectroNeuronElectrophysiologicalFeature ;
    skos:definition "Duration of AP after-hyperpolarization, explictly refered to by author as fast"@en ;
    nsg:units "ms" .

efe:FastAHPVoltage a owl:Class ;
    rdfs:label "Fast AHP Voltage"@en ;
    rdfs:subClassOf bmo:NeuronElectrophysiologicalFeature,
        efe:NeuroElectroNeuronElectrophysiologicalFeature ;
    skos:definition "Calculated as the AHP absolute voltage, explictly refered to by author as fast."@en ;
    nsg:units "mV" .

efe:FiringFrequency a owl:Class ;
    rdfs:label "Firing Frequency"@en ;
    rdfs:subClassOf bmo:NeuronElectrophysiologicalFeature,
        efe:NeuroElectroNeuronElectrophysiologicalFeature ;
    skos:definition "AP discharge rate, AP frequency, spike rate, firing rate, spike frequency, mean firing rate, steady state firing rate, average firing rate, steady firing rate"@en ;
    nsg:units "Hz" .

efe:FirstSpikeLatency a owl:Class ;
    rdfs:label "First Spike Latency"@en ;
    rdfs:subClassOf bmo:NeuronElectrophysiologicalFeature,
        efe:NeuroElectroNeuronElectrophysiologicalFeature ;
    skos:definition "Duration to first AP following a depolarizing current step of fixed amplitude"@en ;
    nsg:units "ms" .

efe:ISICV a owl:Class ;
    rdfs:label "ISI CV"@en ;
    rdfs:subClassOf bmo:NeuronElectrophysiologicalFeature ;
    skos:definition "The coefficient of variation of the ISIs"^^xsd:string ;
    efe:efel_id "ISI_CV"^^xsd:string ;
    efe:efel_namespace "LibV1"^^xsd:string ;
    nsg:units "dimensionless"^^xsd:string .

efe:ISILogSlope a owl:Class ;
    rdfs:label "ISI Log Slope"@en ;
    rdfs:subClassOf bmo:NeuronElectrophysiologicalFeature ;
    skos:definition "The slope of a linear fit to a loglog plot of the ISI values."^^xsd:string ;
    efe:efel_id "ISI_log_slope"^^xsd:string ;
    efe:efel_namespace "LibV5"^^xsd:string ;
    nsg:units "ms"^^xsd:string .

efe:ISISemilogSlope a owl:Class ;
    rdfs:label "ISI Semilog Slope"@en ;
    rdfs:subClassOf bmo:NeuronElectrophysiologicalFeature ;
    skos:definition "The slope of a linear fit to a semilog plot of the  inter-spike interval (ISI) values"^^xsd:string ;
    efe:efel_id "ISI_semilog_slope"^^xsd:string ;
    efe:efel_namespace "LibV5"^^xsd:string ;
    nsg:units "ms"^^xsd:string .

efe:InputResistance a owl:Class ;
    rdfs:label "Input Resistance"@en ;
    rdfs:subClassOf bmo:NeuronElectrophysiologicalFeature,
        efe:NeuroElectroNeuronElectrophysiologicalFeature ;
    skos:definition "Input resistance measured at steady-state voltage response to current injection"@en ;
    nsg:units "M\\ohm" .

efe:InvFifthISI a owl:Class ;
    rdfs:label "Inv Fifth ISI"@en ;
    rdfs:subClassOf bmo:NeuronElectrophysiologicalFeature ;
    skos:definition "1.0 over fith inter-spike interval (ISI); returns 0 when no ISI"^^xsd:string ;
    efe:efel_id "inv_fifth_ISI"^^xsd:string ;
    efe:efel_namespace "LibV5"^^xsd:string ;
    nsg:units "Hz"^^xsd:string .

efe:InvFirstISI a owl:Class ;
    rdfs:label "Inv First ISI"@en ;
    rdfs:subClassOf bmo:NeuronElectrophysiologicalFeature ;
    skos:definition "1.0 over first inter-spike interval (ISI); returns 0 when no ISI"^^xsd:string ;
    efe:efel_id "inv_first_ISI"^^xsd:string ;
    efe:efel_namespace "LibV5"^^xsd:string ;
    nsg:units "Hz"^^xsd:string .

efe:InvFourthISI a owl:Class ;
    rdfs:label "Inv Fourth ISI"@en ;
    rdfs:subClassOf bmo:NeuronElectrophysiologicalFeature ;
    skos:definition "1.0 over fourth inter-spike interval (ISI); returns 0 when no ISI"^^xsd:string ;
    efe:efel_id "inv_fourth_ISI"^^xsd:string ;
    efe:efel_namespace "LibV5"^^xsd:string ;
    nsg:units "Hz"^^xsd:string .

efe:InvLastISI a owl:Class ;
    rdfs:label "Inv Last ISI"@en ;
    rdfs:subClassOf bmo:NeuronElectrophysiologicalFeature ;
    skos:definition "1.0 over last inter-spike interval (ISI); returns 0 when no ISI"^^xsd:string ;
    efe:efel_id "inv_last_ISI"^^xsd:string ;
    efe:efel_namespace "LibV5"^^xsd:string ;
    nsg:units "Hz"^^xsd:string .

efe:InvSecondISI a owl:Class ;
    rdfs:label "Inv Second ISI"@en ;
    rdfs:subClassOf bmo:NeuronElectrophysiologicalFeature ;
    skos:definition "1.0 over second inter-spike interval (ISI); returns 0 when no ISI"^^xsd:string ;
    efe:efel_id "inv_second_ISI"^^xsd:string ;
    efe:efel_namespace "LibV5"^^xsd:string ;
    nsg:units "Hz"^^xsd:string .

efe:InvThirdISI a owl:Class ;
    rdfs:label "Inv Third ISI"@en ;
    rdfs:subClassOf bmo:NeuronElectrophysiologicalFeature ;
    skos:definition "1.0 over third inter-spike interval (ISI); returns 0 when no ISI"^^xsd:string ;
    efe:efel_id "inv_third_ISI"^^xsd:string ;
    efe:efel_namespace "LibV5"^^xsd:string ;
    nsg:units "Hz"^^xsd:string .

efe:InvTimeToFirstSpike a owl:Class ;
    rdfs:label "Inv Time To First Spike"@en ;
    rdfs:subClassOf bmo:NeuronElectrophysiologicalFeature ;
    skos:definition "1.0 over time to first spike; returns 0 when no spike"^^xsd:string ;
    efe:efel_id "inv_time_to_first_spike"^^xsd:string ;
    efe:efel_namespace "LibV5"^^xsd:string .

efe:MaximumFiringRate a owl:Class ;
    rdfs:label "Maximum Firing Rate"@en ;
    rdfs:subClassOf bmo:NeuronElectrophysiologicalFeature,
        efe:NeuroElectroNeuronElectrophysiologicalFeature ;
    skos:definition "Maximum observed AP discharge rate"@en ;
    nsg:units "Hz" .

efe:MaximumVoltage a owl:Class ;
    rdfs:label "Maximum Voltage"@en ;
    rdfs:subClassOf bmo:NeuronElectrophysiologicalFeature ;
    skos:definition "The maximum of the voltage during the stimulus."^^xsd:string ;
    efe:efel_id "maximum_voltage"^^xsd:string ;
    efe:efel_namespace "LibV1"^^xsd:string ;
    nsg:units "mV"^^xsd:string .

efe:MaximumVoltageFromVoltagebase a owl:Class ;
    rdfs:label "Maximum Voltage From Voltagebase"@en ;
    rdfs:subClassOf bmo:NeuronElectrophysiologicalFeature ;
    skos:definition "Difference between maximum voltage during stimulus and voltage base"^^xsd:string ;
    efe:efel_id "maximum_voltage_from_voltagebase"^^xsd:string ;
    efe:efel_namespace "LibV5"^^xsd:string ;
    nsg:units "mV"^^xsd:string .

efe:MeanFrequency a owl:Class ;
    rdfs:label "Mean Frequency"@en ;
    rdfs:subClassOf bmo:NeuronElectrophysiologicalFeature ;
    skos:definition "The mean frequency of the firing rate."^^xsd:string ;
    efe:efel_id "mean_frequency"^^xsd:string ;
    efe:efel_namespace "LibV1"^^xsd:string ;
    nsg:units "Hz"^^xsd:string .

efe:MediumAHPAmplitude a owl:Class ;
    rdfs:label "Medium AHP Amplitude"@en ;
    rdfs:subClassOf bmo:NeuronElectrophysiologicalFeature,
        efe:NeuroElectroNeuronElectrophysiologicalFeature ;
    skos:definition "Calculated as the difference between AP threshold and AP trough, explictly refered to by author as medium"@en ;
    nsg:units "mV" .

efe:MediumAHPAmplitudeFromResting a owl:Class ;
    rdfs:label "Medium AHP Amplitude From Resting"@en ;
    rdfs:subClassOf bmo:NeuronElectrophysiologicalFeature,
        efe:NeuroElectroNeuronElectrophysiologicalFeature ;
    skos:definition "Calculated as the difference between resting or baseline voltages and AP trough, explictly refered to by author as medium"@en ;
    nsg:units "mV" .

efe:MediumAHPDuration a owl:Class ;
    rdfs:label "Medium AHP Duration"@en ;
    rdfs:subClassOf bmo:NeuronElectrophysiologicalFeature,
        efe:NeuroElectroNeuronElectrophysiologicalFeature ;
    skos:definition "Duration of AP after-hyperpolarization, explictly refered to by author as medium"@en ;
    nsg:units "ms" .

efe:MediumAHPVoltage a owl:Class ;
    rdfs:label "Medium AHP Voltage"@en ;
    rdfs:subClassOf bmo:NeuronElectrophysiologicalFeature,
        efe:NeuroElectroNeuronElectrophysiologicalFeature ;
    skos:definition "Calculated as the AHP absolute voltage, explictly refered to by author as medium."@en ;
    nsg:units "mV" .

efe:MembraneTimeConstant a owl:Class ;
    rdfs:label "Membrane Time Constant"@en ;
    rdfs:subClassOf bmo:NeuronElectrophysiologicalFeature,
        efe:NeuroElectroNeuronElectrophysiologicalFeature ;
    skos:definition "Time constant for the membrane to repolarize after a small current injection of fixed amplitude and duration"@en ;
    nsg:units "ms" .

efe:MinimumVoltage a owl:Class ;
    rdfs:label "Minimum Voltage"@en ;
    rdfs:subClassOf bmo:NeuronElectrophysiologicalFeature ;
    skos:definition "The minimum of the voltage during the stimulus."^^xsd:string ;
    efe:efel_id "minimum_voltage"^^xsd:string ;
    efe:efel_namespace "LibV1"^^xsd:string ;
    nsg:units "mV"^^xsd:string .

efe:NumberInitialSpikes a owl:Class ;
    rdfs:label "Number Initial Spikes"@en ;
    rdfs:subClassOf bmo:NeuronElectrophysiologicalFeature ;
    skos:definition "Number of spikes at the beginning of the stimulus"^^xsd:string ;
    efe:efel_id "number_initial_spikes"^^xsd:string ;
    efe:efel_namespace "LibV5"^^xsd:string ;
    nsg:units "dimensionless"^^xsd:string .

efe:OhmicInputResistance a owl:Class ;
    rdfs:label "Ohmic Input Resistance"@en ;
    rdfs:subClassOf bmo:NeuronElectrophysiologicalFeature ;
    skos:definition "The ratio between the voltage deflection and stimulus current."^^xsd:string ;
    efe:efel_id "ohmic_input_resistance"^^xsd:string ;
    efe:efel_namespace "LibV1"^^xsd:string ;
    nsg:units "mV/nA"^^xsd:string .

efe:OhmicInputResistanceVBSSSE a owl:Class ;
    rdfs:label "Ohmic Input Resistance VB SSSE"@en ;
    rdfs:subClassOf bmo:NeuronElectrophysiologicalFeature ;
    skos:definition "The  ratio  between  the  voltage  deflection  (between  voltage  base  and  steady-state  voltage  at  stimend)  and  stimuluscurrent"^^xsd:string ;
    efe:efel_id "ohmic_input_resistance_vb_ssse"^^xsd:string ;
    efe:efel_namespace "LibV5"^^xsd:string ;
    nsg:units "mV/nA"^^xsd:string .

efe:RestingMembranePotential a owl:Class ;
    rdfs:label "Resting Membrane Potential"@en ;
    rdfs:subClassOf bmo:NeuronElectrophysiologicalFeature,
        efe:NeuroElectroNeuronElectrophysiologicalFeature ;
    skos:definition "Membrane potential at the onset of whole-cell recording"@en ;
    nsg:units "mV" .

efe:Rheobase a owl:Class ;
    rdfs:label "Rheobase"@en ;
    rdfs:subClassOf bmo:NeuronElectrophysiologicalFeature,
        efe:NeuroElectroNeuronElectrophysiologicalFeature ;
    skos:definition "Minimum current injected somatically required to fire AP"@en ;
    nsg:units "pA" .

efe:SagAmplitude a owl:Class ;
    rdfs:label "Sag Amplitude1"@en ;
    rdfs:subClassOf bmo:NeuronElectrophysiologicalFeature ;
    skos:definition "The difference between the minimal voltage and the steady state at stimend"^^xsd:string ;
    efe:efel_id "sag_amplitude"^^xsd:string ;
    efe:efel_namespace "LibV5"^^xsd:string ;
    nsg:units "mV"^^xsd:string .

efe:SagAmplitude2 a owl:Class ;
    rdfs:label "Sag Amplitude2"@en ;
    rdfs:subClassOf bmo:NeuronElectrophysiologicalFeature,
        efe:NeuroElectroNeuronElectrophysiologicalFeature ;
    skos:definition "Absolute difference between the steady state decrease in the voltage and the largest decrease in voltage following a hyperpolarizing current step."^^xsd:string ;
    nsg:units "mV"^^xsd:string .

efe:SagRatio a owl:Class ;
    rdfs:label "Sag Ratio"@en ;
    rdfs:subClassOf bmo:NeuronElectrophysiologicalFeature,
        efe:NeuroElectroNeuronElectrophysiologicalFeature ;
    skos:definition "Ratio between the steady state decrease in the voltage and the largest decrease in voltage following a hyperpolarizing current step."@en ;
    nsg:units "Unitless" .

efe:SagRatio1 a owl:Class ;
    rdfs:label "Sag Ratio1"@en ;
    rdfs:subClassOf bmo:NeuronElectrophysiologicalFeature ;
    skos:definition "The ratio between the sag amplitude and the maximal sag extend from voltage base"^^xsd:string ;
    efe:efel_id "sag_ratio1"^^xsd:string ;
    efe:efel_namespace "LibV5"^^xsd:string ;
    nsg:units "dimensionless"^^xsd:string .

efe:SagRatio2 a owl:Class ;
    rdfs:label "Sag Ratio2"@en ;
    rdfs:subClassOf bmo:NeuronElectrophysiologicalFeature ;
    skos:definition "Absolute difference between the steady state decrease in the voltage and the largest decrease in voltage following a hyperpolarizing current step."^^xsd:string ;
    efe:efel_id "sag_ratio2"^^xsd:string ;
    efe:efel_namespace "LibV5"^^xsd:string ;
    nsg:units "dimensionless"^^xsd:string .

efe:SlowAHPAmplitude a owl:Class ;
    rdfs:label "Slow AHP Amplitude"@en ;
    rdfs:subClassOf bmo:NeuronElectrophysiologicalFeature,
        efe:NeuroElectroNeuronElectrophysiologicalFeature ;
    skos:definition "Calculated as the difference between AP threshold and AP trough, explictly refered to by author as slow"@en ;
    nsg:units "mV" .

efe:SlowAHPAmplitudeFromResting a owl:Class ;
    rdfs:label "Slow AHP Amplitude From Resting"@en ;
    rdfs:subClassOf bmo:NeuronElectrophysiologicalFeature,
        efe:NeuroElectroNeuronElectrophysiologicalFeature ;
    skos:definition "Calculated as the difference between resting or baseline voltages and AP trough, explictly refered to by author as slow"@en ;
    nsg:units "mV" .

efe:SlowAHPDuration a owl:Class ;
    rdfs:label "Slow AHP Duration"@en ;
    rdfs:subClassOf bmo:NeuronElectrophysiologicalFeature,
        efe:NeuroElectroNeuronElectrophysiologicalFeature ;
    skos:definition "Duration of AP after-hyperpolarization, explictly refered to by author as slow"@en ;
    nsg:units "ms" .

efe:SlowAHPVoltage a owl:Class ;
    rdfs:label "Slow AHP Voltage"@en ;
    rdfs:subClassOf bmo:NeuronElectrophysiologicalFeature,
        efe:NeuroElectroNeuronElectrophysiologicalFeature ;
    skos:definition "Calculated as the AHP absolute voltage, explictly refered to by author as slow."@en ;
    nsg:units "mV" .

efe:SpikeAmplitude a owl:Class ;
    rdfs:label "Spike Amplitude"@en ;
    rdfs:subClassOf bmo:NeuronElectrophysiologicalFeature,
        efe:NeuroElectroNeuronElectrophysiologicalFeature ;
    skos:definition "Voltage indicating height of action potential. Usually calculated as the difference between AP peak and AP threshold voltages. Commonly measured using first AP in train at rheobase current."@en ;
    nsg:units "mV" .

efe:SpikeAmplitudeFromResting a owl:Class ;
    rdfs:label "Spike Amplitude From Resting"@en ;
    rdfs:subClassOf bmo:NeuronElectrophysiologicalFeature,
        efe:NeuroElectroNeuronElectrophysiologicalFeature ;
    skos:definition "Voltage indicating height of action potential, calculated as the difference between AP peak and resting or baseline voltages. Commonly measured using first AP in train at rheobase current."@en ;
    nsg:units "mV" .

efe:SpikeAmplitudeFromTrough a owl:Class ;
    rdfs:label "Spike Amplitude From Trough"@en ;
    rdfs:subClassOf bmo:NeuronElectrophysiologicalFeature,
        efe:NeuroElectroNeuronElectrophysiologicalFeature ;
    skos:definition "Voltage indicating height of action potential, calculated as the difference between AP peak and AHP trough voltages. Commonly measured using first AP in train at rheobase current."@en ;
    nsg:units "mV" .

efe:SpikeDecayTime a owl:Class ;
    rdfs:label "Spike Decay Time"@en ;
    rdfs:subClassOf bmo:NeuronElectrophysiologicalFeature,
        efe:NeuroElectroNeuronElectrophysiologicalFeature ;
    skos:definition "Time for spike to fall from peak to threshold, usually calculated as 10-90% decay time"@en ;
    nsg:units "ms" .

efe:SpikeHalf-Width a owl:Class ;
    rdfs:label "Spike Half-Width"@en ;
    rdfs:subClassOf bmo:NeuronElectrophysiologicalFeature,
        efe:NeuroElectroNeuronElectrophysiologicalFeature ;
    skos:definition "Calculated as the AP duration at the membrane voltage halfway between AP threshold and AP peak. Most commonly calculated using first AP in train at rheobase. current."@en ;
    nsg:units "ms" .

efe:SpikeMaxDecaySlope a owl:Class ;
    rdfs:label "Spike Max Decay Slope"@en ;
    rdfs:subClassOf bmo:NeuronElectrophysiologicalFeature,
        efe:NeuroElectroNeuronElectrophysiologicalFeature ;
    skos:definition "Maximum rate of rise of membrane voltage during spike falling phase"@en ;
    nsg:units "mV/ms" .

efe:SpikeMaxRiseSlope a owl:Class ;
    rdfs:label "Spike Max Rise Slope"@en ;
    rdfs:subClassOf bmo:NeuronElectrophysiologicalFeature,
        efe:NeuroElectroNeuronElectrophysiologicalFeature ;
    skos:definition "Maximum rate of rise of membrane voltage during spike rising phase"@en ;
    nsg:units "mV/ms" .

efe:SpikePeak a owl:Class ;
    rdfs:label "Spike Peak"@en ;
    rdfs:subClassOf bmo:NeuronElectrophysiologicalFeature,
        efe:NeuroElectroNeuronElectrophysiologicalFeature ;
    skos:definition "Maximum voltage reached during AP"@en ;
    nsg:units "mV" .

efe:SpikeRiseTime a owl:Class ;
    rdfs:label "Spike Rise Time"@en ;
    rdfs:subClassOf bmo:NeuronElectrophysiologicalFeature,
        efe:NeuroElectroNeuronElectrophysiologicalFeature ;
    skos:definition "Time for spike to rise from threshold to peak, usually calculated as 10-90% rise time"@en ;
    nsg:units "ms" .

efe:SpikeThreshold a owl:Class ;
    rdfs:label "Spike Threshold"@en ;
    rdfs:subClassOf bmo:NeuronElectrophysiologicalFeature,
        efe:NeuroElectroNeuronElectrophysiologicalFeature ;
    skos:definition "Voltage at which AP is initiated (as assessed by measuring rising slope of membrane voltage)"@en ;
    nsg:units "mV" .

efe:SpikeWidth a owl:Class ;
    rdfs:label "Spike Width"@en ;
    rdfs:subClassOf bmo:NeuronElectrophysiologicalFeature,
        efe:NeuroElectroNeuronElectrophysiologicalFeature ;
    skos:definition "Duration of AP, not explictly refered to as half-width"@en ;
    nsg:units "ms" .

efe:Spikecount a owl:Class ;
    rdfs:label "Spikecount"@en ;
    rdfs:subClassOf bmo:NeuronElectrophysiologicalFeature ;
    skos:definition "Number of spikes in the trace, including outside of stimulus interval."^^xsd:string ;
    efe:efel_id "Spikecount"^^xsd:string ;
    efe:efel_namespace "LibV1"^^xsd:string ;
    nsg:units "dimensionless"^^xsd:string .

efe:SpikecountStimint a owl:Class ;
    rdfs:label "Spikecount Stimint"@en ;
    rdfs:subClassOf bmo:NeuronElectrophysiologicalFeature ;
    skos:definition "Number of spikes inside the stimulus interval"^^xsd:string ;
    efe:efel_id "Spikecount_stimint"^^xsd:string ;
    efe:efel_namespace "LibV5"^^xsd:string ;
    nsg:units "dimensionless"^^xsd:string .

efe:SpontaneousFiringRate a owl:Class ;
    rdfs:label "Spontaneous Firing Rate"@en ;
    rdfs:subClassOf bmo:NeuronElectrophysiologicalFeature,
        efe:NeuroElectroNeuronElectrophysiologicalFeature ;
    skos:definition "AP discharge rate in the absence of current injection or a stimulus"@en ;
    nsg:units "Hz" .

efe:SteadyStateVoltage a owl:Class ;
    rdfs:label "Steady State Voltage"@en ;
    rdfs:subClassOf bmo:NeuronElectrophysiologicalFeature ;
    skos:definition "The average voltage after the stimulus."^^xsd:string ;
    efe:efel_id "steady_state_voltage"^^xsd:string ;
    efe:efel_namespace "LibV1"^^xsd:string ;
    nsg:units "mV"^^xsd:string .

efe:SteadyStateVoltageStimend a owl:Class ;
    rdfs:label "Steady State Voltage Stimend"@en ;
    rdfs:subClassOf bmo:NeuronElectrophysiologicalFeature ;
    skos:definition "The average voltage during the last 10% of the stimulus duration."^^xsd:string ;
    efe:efel_id "steady_state_voltage_stimend"^^xsd:string ;
    efe:efel_namespace "LibV5"^^xsd:string ;
    nsg:units "mV"^^xsd:string .

efe:TimeToFirstSpike a owl:Class ;
    rdfs:label "Time To First Spike"@en ;
    rdfs:subClassOf bmo:NeuronElectrophysiologicalFeature ;
    skos:definition "Time from the start of the stimulus to the maximum of the first peak."^^xsd:string ;
    efe:efel_id "time_to_first_spike"^^xsd:string ;
    efe:efel_namespace "LibV1"^^xsd:string ;
    nsg:units "ms"^^xsd:string .

efe:TimeToLastSpike a owl:Class ;
    rdfs:label "Time To Last Spike"@en ;
    rdfs:subClassOf bmo:NeuronElectrophysiologicalFeature ;
    skos:definition "Time from stimulus start to last spike"^^xsd:string ;
    efe:efel_id "time_to_last_spike"^^xsd:string ;
    efe:efel_namespace "LibV5"^^xsd:string ;
    nsg:units "ms"^^xsd:string .

efe:TimeToSecondSpike a owl:Class ;
    rdfs:label "Time To Second Spike"@en ;
    rdfs:subClassOf bmo:NeuronElectrophysiologicalFeature ;
    skos:definition "Time from the start of the stimulus to the maximum of the second peak"^^xsd:string ;
    efe:efel_id "time_to_second_spike"^^xsd:string ;
    efe:efel_namespace "LibV5"^^xsd:string ;
    nsg:units "ms"^^xsd:string .

efe:VoltageAfterStim a owl:Class ;
    rdfs:label "Voltage After Stim"@en ;
    rdfs:subClassOf bmo:NeuronElectrophysiologicalFeature ;
    skos:definition "The mean voltage after the stimulus in (stim_end + 25%*end_period, stim_end + 75%*end_period)"^^xsd:string ;
    efe:efel_id "voltage_after_stim"^^xsd:string ;
    efe:efel_namespace "LibV5"^^xsd:string ;
    nsg:units "mV"^^xsd:string .

efe:VoltageBase a owl:Class ;
    rdfs:label "Voltage Base"@en ;
    rdfs:subClassOf bmo:NeuronElectrophysiologicalFeature ;
    skos:definition "The average voltage during the last 10% of time before the stimulus."^^xsd:string ;
    efe:efel_id "voltage_base"^^xsd:string ;
    efe:efel_namespace "LibV5"^^xsd:string ;
    nsg:units "mV"^^xsd:string .

efe:VoltageDeflection a owl:Class ;
    rdfs:label "Voltage Deflection"@en ;
    rdfs:subClassOf bmo:NeuronElectrophysiologicalFeature ;
    skos:definition "The voltage deflection between voltage base and steady-state voltage at stimend. The voltage base used is the average voltage during all of the time before the stimulus and the steady state voltage at stimend used is the average voltage of the five values before the last five values before the end of the stimulus duration."^^xsd:string ;
    efe:efel_id "voltage_deflection"^^xsd:string ;
    efe:efel_namespace "LibV1"^^xsd:string ;
    nsg:units "mV"^^xsd:string .

efe:VoltageDeflectionBegin a owl:Class ;
    rdfs:label "Voltage Deflection Begin"@en ;
    rdfs:subClassOf bmo:NeuronElectrophysiologicalFeature ;
    skos:definition "The voltage deflection between voltage base and steady-state voltage soon after stimulation start. The voltage base used is the average voltage during all of the time before the stimulus and the steady state voltage used is the average voltage taken from 5% to 15% of the stimulus duration."^^xsd:string ;
    efe:efel_id "voltage_deflection_begin"^^xsd:string ;
    efe:efel_namespace "LibV5"^^xsd:string .

efe:VoltageDeflectionVBSSSE a owl:Class ;
    rdfs:label "Voltage Deflection VB SSSE"@en ;
    rdfs:subClassOf bmo:NeuronElectrophysiologicalFeature ;
    skos:definition "The voltage deflection between voltage base and steady-state voltage at stimend. The voltage base used is the average voltage during the last 10% of time before the stimulus and the steady statevoltage at stimend used is the average voltage during the last 10% of the stimulus duration"^^xsd:string ;
    efe:efel_id "voltage_deflection_vb_ssse"^^xsd:string ;
    efe:efel_namespace "LibV5"^^xsd:string ;
    nsg:units "mV"^^xsd:string .

efe:efel_id a owl:AnnotationProperty ;
    rdfs:label "efel_id"@en .

efe:efel_namespace a owl:AnnotationProperty ;
    rdfs:label "efel_namespace"@en .

nsg:units a owl:AnnotationProperty ;
    rdfs:label "units"@en .

efe:NeuroElectroNeuronElectrophysiologicalFeature a owl:Class ;
    rdfs:label "NeuroElectro Neuron Electrophysiological Feature"@en .

bmo:NeuronElectrophysiologicalFeature a owl:Class ;
    rdfs:label "Neuron Electrophysiological Feature"@en .

